add nbe tests

tests/bug-reports/Bug2699.fst
@@ -129,3 +129,115 @@ let testu128_lt = assert FStar.UInt128.(uint_to_t 29 `lt` uint_to_t 30)
 let testu128_lte = assert FStar.UInt128.(uint_to_t 30 `lte` uint_to_t 30)
             by (norm [primops]; trivial(); qed())
 
+
+
+let nbe_testu8_add_mod = assert FStar.UInt8.(250uy `add_mod` 6uy == 0uy)
+            by (norm [nbe;primops]; trefl(); qed())
+
+let nbe_testu8_sub_mod = assert FStar.UInt8.(6uy `sub_mod` 250uy == 12uy)
+            by (norm [nbe;primops]; trefl(); qed())
+
+let nbe_testu8_mul_mod = assert FStar.UInt8.(30uy `mul_mod` 12uy == 104uy)
+            by (norm [nbe;primops]; trefl(); qed())
+
+let nbe_testu8_gt = assert FStar.UInt8.(30uy `gt` 10uy)
+            by (norm [nbe;primops]; trivial(); qed())
+
+let nbe_testu8_gte = assert FStar.UInt8.(30uy `gte` 30uy)
+            by (norm [nbe;primops]; trivial(); qed())
+
+let nbe_testu8_lt = assert FStar.UInt8.(29uy `lt` 30uy)
+            by (norm [nbe;primops]; trivial(); qed())
+
+let nbe_testu8_lte = assert FStar.UInt8.(30uy `lte` 30uy)
+            by (norm [nbe;primops]; trivial(); qed())
+
+
+let nbe_testu16_add_mod = assert FStar.UInt16.(65530us `add_mod` 6us == 0us)
+            by (norm [nbe;primops]; trefl(); qed())
+
+let nbe_testu16_sub_mod = assert FStar.UInt16.(6us `sub_mod` 65530us == 12us)
+            by (norm [nbe;primops]; trefl(); qed())
+
+let nbe_testu16_mul_mod = assert FStar.UInt16.((256us `mul_mod` 256us) == 0us)
+            by (norm [nbe;primops]; trefl(); qed())
+
+let nbe_testu16_gt = assert FStar.UInt16.(30us `gt` 10us)
+            by (norm [nbe;primops]; trivial(); qed())
+
+let nbe_testu16_gte = assert FStar.UInt16.(30us `gte` 30us)
+            by (norm [nbe;primops]; trivial(); qed())
+
+let nbe_testu16_lt = assert FStar.UInt16.(29us `lt` 30us)
+            by (norm [nbe;primops]; trivial(); qed())
+
+let nbe_testu16_lte = assert FStar.UInt16.(30us `lte` 30us)
+            by (norm [nbe;primops]; trivial(); qed())
+
+
+let nbe_testu32_add_mod = assert FStar.UInt32.(0xfffffffaul `add_mod` 6ul == 0ul)
+            by (norm [nbe;primops]; trefl(); qed())
+
+let nbe_testu32_sub_mod = assert FStar.UInt32.(6ul `sub_mod` 0xfffffffaul == 12ul)
+            by (norm [nbe;primops]; trefl(); qed())
+
+let nbe_testu32_mul_mod = assert FStar.UInt32.((0x10000ul `mul_mod` 0x10000ul) == 0ul)
+            by (norm [nbe;primops]; trefl(); qed())
+
+let nbe_testu32_gt = assert FStar.UInt32.(30ul `gt` 10ul)
+            by (norm [nbe;primops]; trivial(); qed())
+
+let nbe_testu32_gte = assert FStar.UInt32.(30ul `gte` 30ul)
+            by (norm [nbe;primops]; trivial(); qed())
+
+let nbe_testu32_lt = assert FStar.UInt32.(29ul `lt` 30ul)
+            by (norm [nbe;primops]; trivial(); qed())
+
+let nbe_testu32_lte = assert FStar.UInt32.(30ul `lte` 30ul)
+            by (norm [nbe;primops]; trivial(); qed())
+
+
+let nbe_testu64_add_mod = assert FStar.UInt64.(0xfffffffffffffffauL `add_mod` 6uL == 0uL)
+            by (norm [nbe;primops]; trefl(); qed())
+
+let nbe_testu64_sub_mod = assert FStar.UInt64.(6uL `sub_mod` 0xfffffffffffffffauL == 12uL)
+            by (norm [nbe;primops]; trefl(); qed())
+
+let nbe_testu64_muL_mod = assert FStar.UInt64.((0x100000000uL `mul_mod` 0x100000000uL) == 0uL)
+            by (norm [nbe;primops]; trefl(); qed())
+
+let nbe_testu64_gt = assert FStar.UInt64.(30uL `gt` 10uL)
+            by (norm [nbe;primops]; trivial(); qed())
+
+let nbe_testu64_gte = assert FStar.UInt64.(30uL `gte` 30uL)
+            by (norm [nbe;primops]; trivial(); qed())
+
+let nbe_testu64_lt = assert FStar.UInt64.(29uL `lt` 30uL)
+            by (norm [nbe;primops]; trivial(); qed())
+
+let nbe_testu64_lte = assert FStar.UInt64.(30uL `lte` 30uL)
+            by (norm [nbe;primops]; trivial(); qed())
+
+
+let nbe_testu128_add_mod = assert FStar.UInt128.(uint_to_t 0xfffffffffffffffffffffffffffffffa `add_mod` uint_to_t 6 == uint_to_t 0)
+            by (norm [nbe;primops]; trefl(); qed())
+
+let nbe_testu128_sub_mod = assert FStar.UInt128.(uint_to_t 6 `sub_mod` uint_to_t 0xfffffffffffffffffffffffffffffffa == uint_to_t 12)
+            by (norm [nbe;primops]; trefl(); qed())
+
+// No mul_mod for 128
+// let nbe_testu128_muL_mod = assert FStar.UInt128.((uint_to_t 0x1000000000000 `mul_mod` uint_to_t 0x1000000000000) == uint_to_t 0)
+//             by (norm [nbe;primops]; trefl(); qed())
+
+let nbe_testu128_gt = assert FStar.UInt128.(uint_to_t 30 `gt` uint_to_t 10)
+            by (norm [nbe;primops]; trivial(); qed())
+
+let nbe_testu128_gte = assert FStar.UInt128.(uint_to_t 30 `gte` uint_to_t 30)
+            by (norm [nbe;primops]; trivial(); qed())
+
+let nbe_testu128_lt = assert FStar.UInt128.(uint_to_t 29 `lt` uint_to_t 30)
+            by (norm [nbe;primops]; trivial(); qed())
+
+let nbe_testu128_lte = assert FStar.UInt128.(uint_to_t 30 `lte` uint_to_t 30)
+            by (norm [nbe;primops]; trivial(); qed())
+
